fstar/new/MLS.TreeDEM.Welcome.fst
@@ -1,0 +1,253 @@
+module MLS.TreeDEM.Welcome
+
+open Lib.ByteSequence
+open MLS.NetworkTypes
+open MLS.NetworkBinder
+open MLS.Parser
+open MLS.Crypto
+open MLS.Tree
+open MLS.TreeSync.Types
+open MLS.TreeDEM.Keys
+open MLS.Result
+
+noeq type welcome_group_info = {
+  group_id: bytes;
+  epoch: nat;
+  tree_hash: bytes;
+  confirmed_transcript_hash: bytes;
+  extensions: bytes;
+  confirmation_tag: bytes;
+  signer_index: nat;
+  signature: bytes;
+}
+
+noeq type group_secrets = {
+  joiner_secret: bytes;
+  path_secret: option bytes;
+  psks: option pre_shared_keys_nt;
+}
+
+//TODO: move in Crypto? (copy-pasted from TreeKEM)
+noeq type hpke_ciphertext = {
+  kem_output: bytes;
+  ciphertext: bytes;
+}
+
+noeq type encrypted_group_secrets = {
+  key_package_hash: bytes;
+  enc_group_secrets: hpke_ciphertext
+}
+
+noeq type welcome = {
+  //version ?
+  //cipher_suite ?
+  secrets: list encrypted_group_secrets;
+  encrypted_group_info: bytes;
+}
+
+(*** From / to network ***)
+
+val network_to_welcome_group_info: group_info_nt -> welcome_group_info
+let network_to_welcome_group_info gi =
+  {
+    group_id = gi.group_id;
+    epoch = Lib.IntTypes.v gi.epoch;
+    tree_hash = gi.tree_hash;
+    confirmed_transcript_hash = gi.confirmed_transcript_hash;
+    extensions = gi.extensions;
+    confirmation_tag = gi.confirmation_tag.mac_value;
+    signer_index = Lib.IntTypes.v gi.signer_index;
+    signature = gi.signature;
+  }
+
+val welcome_group_info_to_network: welcome_group_info -> result group_info_nt
+let welcome_group_info_to_network gi =
+  if not (Seq.length gi.group_id < 256) then
+    internal_failure "welcome_group_info_to_network: group_id too long"
+  else if not (gi.epoch < pow2 64) then
+    internal_failure "welcome_group_info_to_network: epoch too big"
+  else if not (Seq.length gi.tree_hash < 256) then
+    internal_failure "welcome_group_info_to_network: tree_hash too long"
+  else if not (Seq.length gi.confirmed_transcript_hash < 256) then
+    internal_failure "welcome_group_info_to_network: confirmed_transcript_hash too long"
+  else if not (Seq.length gi.extensions < pow2 32) then
+    internal_failure "welcome_group_info_to_network: extensions too long"
+  else if not (Seq.length gi.confirmation_tag < 255) then
+    internal_failure "welcome_group_info_to_network: confirmation_tag too long"
+  else if not (gi.signer_index < pow2 32) then
+    internal_failure "welcome_group_info_to_network: signer_index too big"
+  else if not (Seq.length gi.signature < pow2 16) then
+    internal_failure "welcome_group_info_to_network: signature_id too long"
+  else
+    return ({
+      group_id = gi.group_id;
+      epoch = Lib.IntTypes.u64 gi.epoch;
+      tree_hash = gi.tree_hash;
+      confirmed_transcript_hash = gi.confirmed_transcript_hash;
+      extensions = gi.extensions;
+      confirmation_tag = {mac_value = gi.confirmation_tag};
+      signer_index = Lib.IntTypes.u32 gi.signer_index;
+      signature = gi.signature;
+    } <: group_info_nt)
+
+val network_to_group_secrets: group_secrets_nt -> result group_secrets
+let network_to_group_secrets gs =
+  path_secret <-- network_to_option gs.path_secret;
+  psks <-- network_to_option gs.psks;
+  return ({
+    joiner_secret = gs.joiner_secret;
+    path_secret = (
+      match path_secret with
+      | None -> None
+      | Some p -> Some p.path_secret
+    );
+    psks = psks;
+  })
+
+val group_secrets_to_network: group_secrets -> result group_secrets_nt
+let group_secrets_to_network gs =
+  path_secret <-- (
+    match gs.path_secret with
+    | None -> return None_nt
+    | Some p -> (
+      if not (Seq.length p < 256) then
+        internal_failure ""
+      else
+        return (Some_nt ({ path_secret = p } <: path_secret_nt))
+    )
+  );
+  if not (1 <= Seq.length gs.joiner_secret) then
+    internal_failure "group_secrets_to_network: joiner_secret too short"
+  else if not (Seq.length gs.joiner_secret < 256) then
+    internal_failure "group_secrets_to_network: joiner_secret too long"
+  else
+    return ({
+      joiner_secret = gs.joiner_secret;
+      path_secret = path_secret;
+      psks = option_to_network gs.psks;
+    } <: group_secrets_nt)
+
+val network_to_hpke_ciphertext: hpke_ciphertext_nt -> hpke_ciphertext
+let network_to_hpke_ciphertext x =
+  ({
+    kem_output = x.kem_output;
+    ciphertext = x.ciphertext;
+  })
+
+val hpke_ciphertext_to_network: hpke_ciphertext -> result hpke_ciphertext_nt
+let hpke_ciphertext_to_network x =
+  if not (Seq.length x.kem_output < pow2 16) then
+    internal_failure "hpke_ciphertext_to_network: kem_output too long"
+  else if not (Seq.length x.ciphertext < pow2 16) then
+    internal_failure "hpke_ciphertext_to_network: ciphertext too long"
+  else
+    return ({
+      kem_output = x.kem_output;
+      ciphertext = x.ciphertext
+    } <: hpke_ciphertext_nt)
+
+val network_to_encrypted_group_secrets: encrypted_group_secrets_nt -> encrypted_group_secrets
+let network_to_encrypted_group_secrets egs =
+  ({
+    key_package_hash = egs.key_package_hash;
+    enc_group_secrets = network_to_hpke_ciphertext egs.encrypted_group_secrets;
+  })
+
+val encrypted_group_secrets_to_network: encrypted_group_secrets -> result encrypted_group_secrets_nt
+let encrypted_group_secrets_to_network egs =
+  if not (1 <= Seq.length egs.key_package_hash) then
+    internal_failure "encrypted_group_secrets_to_network: key_package_hash too short"
+  else if not (Seq.length egs.key_package_hash < 256) then
+    internal_failure "encrypted_group_secrets_to_network: key_package_hash too long"
+  else (
+    encrypted_group_secrets <-- hpke_ciphertext_to_network egs.enc_group_secrets;
+    return ({
+      key_package_hash = egs.key_package_hash;
+      encrypted_group_secrets = encrypted_group_secrets;
+    } <: encrypted_group_secrets_nt)
+  )
+
+val network_to_welcome: welcome_nt -> welcome
+let network_to_welcome w =
+  {
+    secrets = List.Tot.map network_to_encrypted_group_secrets (Seq.seq_to_list w.secrets);
+    encrypted_group_info = w.encrypted_group_info;
+  }
+
+val welcome_to_network: ciphersuite -> welcome -> result welcome_nt
+let welcome_to_network cs w =
+  secrets <-- mapM encrypted_group_secrets_to_network w.secrets;
+  cipher_suite <-- ciphersuite_to_nt cs;
+  Seq.lemma_list_seq_bij secrets;
+  if not (1 <= Seq.length w.encrypted_group_info) then
+    internal_failure "welcome_to_network: encrypted_group_info too short"
+  else if not (Seq.length w.encrypted_group_info < pow2 32) then
+    internal_failure "welcome_to_network: encrypted_group_info too long"
+  else if not (byte_length ps_encrypted_group_secrets secrets < pow2 32) then
+    internal_failure "welcome_to_network: secrets too long"
+  else (
+    return ({
+      version = PV_mls10;
+      cipher_suite = cipher_suite;
+      secrets = Seq.seq_of_list secrets;
+      encrypted_group_info = w.encrypted_group_info;
+    } <: welcome_nt)
+  )
+
+(*** Utility functions ***)
+
+val hash_leaf_package: cs:ciphersuite -> leaf_package_t -> result (lbytes (hash_length cs))
+let hash_leaf_package cs lp =
+  kp <-- treesync_to_keypackage cs lp;
+  let kp_bytes = ps_key_package.serialize kp in
+  hash_hash cs kp_bytes
+
+val bytes_to_kem_output: cs:ciphersuite -> bytes -> result (hpke_kem_output cs)
+let bytes_to_kem_output cs b =
+  if not (Seq.length b = hpke_kem_output_length cs) then
+    error "bytes_to_kem_output: kem_output has wrong length"
+  else
+    return b
+
+val welcome_secret_to_key: cs:ciphersuite -> bytes -> result (aead_key cs)
+let welcome_secret_to_key cs welcome_secret =
+  kdf_expand cs welcome_secret (string_to_bytes "key") (aead_key_length cs)
+
+val welcome_secret_to_nonce: cs:ciphersuite -> bytes -> result (aead_nonce cs)
+let welcome_secret_to_nonce cs welcome_secret =
+  kdf_expand cs welcome_secret (string_to_bytes "nonce") (aead_nonce_length cs)
+
+(*** Decrypting a welcome ***)
+
+val find_my_encrypted_group_secret: bytes -> list encrypted_group_secrets -> option hpke_ciphertext
+let rec find_my_encrypted_group_secret kp_hash l =
+  match l with
+  | [] -> None
+  | h::t -> (
+    if (h.key_package_hash = kp_hash) then
+      Some h.enc_group_secrets
+    else
+      find_my_encrypted_group_secret kp_hash t
+  )
+
+val decrypt_welcome: cs:ciphersuite -> welcome -> leaf_package_t -> hpke_private_key cs -> option (l:nat & n:tree_size l & treesync l n) -> result (welcome_group_info & group_secrets)
+let decrypt_welcome cs w lp sk opt_tree =
+  group_secrets <-- (
+    my_kp_hash <-- hash_leaf_package cs lp;
+    my_hpke_ciphertext <-- from_option "decrypt_welcome: can't find my encrypted secret" (find_my_encrypted_group_secret my_kp_hash w.secrets);
+    kem_output <-- bytes_to_kem_output cs my_hpke_ciphertext.kem_output;
+    group_secrets_bytes <-- hpke_decrypt cs kem_output sk bytes_empty bytes_empty my_hpke_ciphertext.ciphertext;
+    group_secrets_network <-- from_option "decrypt_welcome: malformed group secrets" ((ps_to_pse ps_group_secrets).parse_exact group_secrets_bytes);
+    network_to_group_secrets group_secrets_network
+  );
+  group_info <-- (
+    welcome_secret <-- secret_joiner_to_welcome cs group_secrets.joiner_secret bytes_empty (*TODO psk*);
+    welcome_key <-- welcome_secret_to_key cs welcome_secret;
+    welcome_nonce <-- welcome_secret_to_nonce cs welcome_secret;
+    group_info_bytes <-- aead_decrypt cs welcome_key welcome_nonce bytes_empty w.encrypted_group_info;
+    group_info_network <-- from_option "decrypt_welcome: malformed group info" ((ps_to_pse ps_group_info).parse_exact group_info_bytes);
+    return (network_to_welcome_group_info group_info_network)
+  );
+  //TODO: integrity check, this is where `opt_tree` will be useful
+  return (group_info, group_secrets)
+
